New "Hybrid Ghost Heap" abstraction for building the interop program logic

theories/interop/gctoken.v
@@ -7,7 +7,7 @@ From iris.proofmode Require Import proofmode.
 From melocoton.c_interface Require Export defs resources.
 From melocoton.ml_lang Require Import lang_instantiation.
 From melocoton.ml_lang Require Export lang primitive_laws.
-From melocoton.interop Require Import basics_resources.
+From melocoton.interop Require Import basics_resources hybrid_ghost_heap.
 
 (** The [GC θ] resource.
 
@@ -55,29 +55,19 @@ Context `{!heapG_ML Σ, !heapG_C Σ}.
 Context `{!wrapperGCtokG Σ}.
 
 Definition GC (θ : addr_map) : iProp Σ :=
-  ∃ (ζ ζfreeze ζσ ζvirt : lstore) (χ χvirt : lloc_map) (σMLvirt : store)
+  ∃ (ζ : lstore) (χ : lloc_map) (σMLvirt : store)
     (roots_s : gset addr) (roots_m : gmap addr lval),
     "GCζ" ∷ ghost_var wrapperG_γζ (1/2) ζ
   ∗ "GCχ" ∷ ghost_var wrapperG_γχ (1/2) χ
   ∗ "GCθ" ∷ ghost_var wrapperG_γθ (1/2) θ
-  ∗ "GCroots" ∷ ghost_var wrapperG_γroots_set (1/2) roots_s
+  ∗ "GCHGH" ∷ HGH χ (Some σMLvirt) ζ
   ∗ "GCinit" ∷ ghost_var wrapperG_γat_init (1/2) false
-  ∗ "GCζvirt" ∷ lstore_own_auth ζvirt
-  ∗ "GCσMLv" ∷ state_interp (σMLvirt : language.language.state ML_lang)
-  ∗ "GCχvirt" ∷ lloc_own_auth χvirt
-  ∗ "GCχNone" ∷ ([∗ map] _↦ℓ ∈ pub_locs_in_lstore χvirt ζvirt, ℓ ↦M/)
+  ∗ "GCroots" ∷ ghost_var wrapperG_γroots_set (1/2) roots_s
   ∗ "GCrootsm" ∷ ghost_map_auth wrapperG_γroots_map 1 roots_m
   ∗ "GCrootspto" ∷ ([∗ map] a ↦ v ∈ roots_m, ∃ w, a ↦C w ∗ ⌜repr_lval θ v w⌝)
   ∗ "%Hrootsdom" ∷ ⌜dom roots_m = roots_s⌝
   ∗ "%Hrootslive" ∷ ⌜roots_are_live θ roots_m⌝
-  ∗ "%Hfreezeρ" ∷ ⌜freeze_lstore ζ ζfreeze⌝
-  ∗ "%Hfreezeeq" ∷ ⌜ζfreeze = ζσ ∪ ζvirt⌝
-  ∗ "%Hfreezedj" ∷ ⌜ζσ ##ₘ ζvirt⌝
-  ∗ "%Hstore_blocks" ∷ ⌜is_store_blocks χvirt σMLvirt ζσ⌝
-  ∗ "%Hother_blocks" ∷ ⌜dom ζvirt ⊆ dom χvirt⌝
-  ∗ "%Hstore" ∷ ⌜is_store χvirt ζfreeze σMLvirt⌝
-  ∗ "%Hχvirt" ∷ ⌜expose_llocs χ χvirt⌝
-  ∗ "%HGCOK" ∷ ⌜GC_correct ζfreeze θ⌝.
+  ∗ "%HGCOK" ∷ ⌜GC_correct ζ θ⌝.
 
 Definition at_init := ghost_var wrapperG_γat_init (1/2) true.
 
