theories/interop/hybrid_ghost_heap.v
@@ -1,0 +1,506 @@
+From Coq Require Import ssreflect.
+From stdpp Require Import strings gmap.
+From transfinite.base_logic.lib Require Import ghost_map ghost_var gen_heap.
+From iris.algebra Require Import gset.
+From iris.proofmode Require Import proofmode.
+From melocoton Require Import named_props.
+From melocoton.ml_lang Require Import lang primitive_laws.
+From melocoton.interop Require Export basics basics_resources.
+
+Section HGH.
+Context `{SI: indexT}.
+Context {Σ : gFunctors}.
+Context `{!heapG_ML Σ, !heapG_C Σ}.
+Context `{!wrapperBasicsG Σ}.
+
+Local Ltac not_elem_of_dom :=
+  repeat lazymatch goal with
+  | H : _ !! _ = None |- _ => apply not_elem_of_dom in H
+  | |- _ !! _ = None => apply not_elem_of_dom
+  end; set_solver.
+
+Definition lstore_hybrid_repr (χ : lloc_map) (ζfreeze : lstore) (σ : store) (ζ : lstore) :=
+  ∃ ζσ,
+    ζfreeze = ζσ ∪ ζ
+  ∧ ζσ ##ₘ ζ
+  ∧ is_store_blocks χ σ ζσ
+  ∧ is_store χ ζfreeze σ.
+
+Lemma lstore_hybrid_repr_refl χ ζ :
+  lstore_hybrid_repr χ ζ ∅ ζ.
+Proof using.
+  exists ∅. split_and!.
+  - rewrite left_id_L//.
+  - apply map_disjoint_dom. set_solver.
+  - split; set_solver.
+  - intros ?. set_solver.
+Qed.
+
+Lemma lstore_hybrid_repr_lookup_loc χ ζfreeze σ ζ ℓ vs γ :
+  lstore_hybrid_repr χ ζfreeze σ ζ →
+  lloc_map_inj χ →
+  σ !! ℓ = Some (Some vs) →
+  χ !! γ = Some (LlocPublic ℓ) →
+  ∃ lvs, ζfreeze !! γ = Some (Bvblock (Mut, (TagDefault, lvs))) ∧
+         Forall2 (is_val χ ζfreeze) vs lvs.
+Proof using.
+  intros (ζσ & Hfreezeeq & ? & Hstore_blocks & Hstore) Hχinj Hσ Hχ.
+  edestruct is_store_blocks_has_loc as (ll & Hlχ & Hγζ);
+    [apply Hstore_blocks|apply Hσ|..].
+  assert (ll = γ) as -> by (eapply Hχinj; eauto). clear Hlχ.
+  apply elem_of_dom in Hγζ. destruct Hγζ as [bb Hζσγ].
+  assert (ζfreeze !! γ = Some bb) as Hfreezell.
+  1: { rewrite Hfreezeeq. by apply lookup_union_Some_l. }
+  unfold is_store in Hstore.
+  specialize (Hstore ℓ vs γ bb Hσ Hχ Hfreezell) as Hstorel.
+  inversion Hstorel; subst vs0 bb. eauto.
+Qed.
+
+Lemma block_sim_arr_of_auth' χ ζfreeze σ ζ vs lvs :
+  lstore_hybrid_repr χ ζfreeze σ ζ →
+  Forall2 (is_val χ ζfreeze) vs lvs →
+  lloc_own_auth χ -∗
+  lstore_own_auth ζ -∗
+  lvs ~~∗ vs.
+Proof using.
+  intros (?&?&?&?&?) ?. eapply block_sim_arr_of_auth; eauto.
+Qed.
+
+Lemma block_sim_arr_auth_is_val' χ ζfreeze σ ζ lvs vs :
+  lstore_hybrid_repr χ ζfreeze σ ζ →
+  lloc_own_auth χ -∗
+  lstore_own_auth ζ -∗
+  lvs ~~∗ vs -∗
+  ⌜Forall2 (is_val χ ζfreeze) vs lvs⌝.
+Proof using.
+  intros (?&->&?&?&?). iApply block_sim_arr_auth_is_val; eauto.
+Qed.
+
+Lemma lstore_hybrid_repr_ml_to_mut χ ζfreeze σ ζ ℓ γ vs lvs :
+  lloc_map_inj χ →
+  χ !! γ = Some (LlocPublic ℓ) →
+  ζfreeze !! γ = Some (Bvblock (Mut, (TagDefault, lvs))) →
+  σ !! ℓ = Some (Some vs) →
+  ζ !! γ = None →
+  lstore_hybrid_repr χ ζfreeze σ ζ →
+  lstore_hybrid_repr χ ζfreeze (<[ℓ:=None]> σ)
+    (<[γ:=Bvblock (Mut, (TagDefault, lvs))]> ζ).
+Proof using.
+  intros Hχinj ? Hfγ ? ? (ζσ & -> & ? & ? & ?).
+  exists (delete γ ζσ). split_and!.
+  - symmetry. apply union_delete_insert.
+    by apply lookup_union_Some_inv_l in Hfγ.
+  - apply map_disjoint_insert_r_2. 1: apply lookup_delete.
+    by apply map_disjoint_delete_l.
+  - eapply is_store_blocks_discard_loc; eauto.
+  - eapply is_store_discard_loc; eauto.
+Qed.
+
+Lemma lstore_hybrid_repr_mut_to_ml χ ζfreeze σ ζ ℓ vs γ lvs :
+  lloc_map_inj χ →
+  χ !! γ = Some (LlocPublic ℓ) →
+  σ !! ℓ = Some None →
+  ζ !! γ = Some (Bvblock (Mut, (TagDefault, lvs))) →
+  Forall2 (is_val χ ζfreeze) vs lvs →
+  lstore_hybrid_repr χ ζfreeze σ ζ →
+  lstore_hybrid_repr χ ζfreeze (<[ℓ:=Some vs]> σ) (delete γ ζ).
+Proof using.
+  intros ? ? ? ? ? (ζσ&->&?&?&?).
+  exists (<[γ:=Bvblock (Mut, (TagDefault, lvs))]> ζσ). split_and!.
+  - erewrite (union_insert_delete ζσ ζ). 2: eapply map_disjoint_Some_r. all: eauto.
+  - apply map_disjoint_insert_l_2. 1: apply lookup_delete.
+    by apply map_disjoint_delete_r.
+  - eapply is_store_blocks_restore_loc; eauto.
+  - eapply is_store_restore_loc; eauto. 1: eapply lookup_union_Some_r; eauto.
+    by constructor.
+Qed.
+
+Lemma lstore_hybrid_repr_lookup_lloc χ ζfreeze σ ζ γ blk :
+  lstore_hybrid_repr χ ζfreeze σ ζ →
+  ζ !! γ = Some blk →
+  ζfreeze !! γ = Some blk.
+Proof using. intros (ζσ&->&?&?&?) ?. by simplify_map_eq. Qed.
+
+Lemma lstore_hybrid_repr_lstore_sub χ ζfreeze σ ζ :
+  lstore_hybrid_repr χ ζfreeze σ ζ →
+  ζ ⊆ ζfreeze.
+Proof using. intros (ζσ&->&?&?&?). by eapply map_union_subseteq_r. Qed.
+
+Lemma lstore_hybrid_repr_expose_lloc χ ζfreeze σ ζ γ :
+  lloc_map_inj χ →
+  χ !! γ = Some LlocPrivate →
+  lstore_hybrid_repr χ ζfreeze σ ζ →
+  ∃ ℓ, ℓ ∉ lloc_map_pub_locs χ ∧
+       ℓ ∉ dom σ ∧
+       lstore_hybrid_repr (<[γ:=LlocPublic ℓ]> χ) ζfreeze (<[ℓ:=None]> σ) ζ.
+Proof using.
+  intros ? ? (ζσ&->&?&Hstore_blocks&?).
+  pose (fresh_locs (lloc_map_pub_locs χ)) as ℓ. exists ℓ.
+  assert (ℓ ∉ lloc_map_pub_locs χ).
+  { intros Hℓ. apply (fresh_locs_fresh (lloc_map_pub_locs χ) 0 ltac:(lia)).
+    rewrite /loc_add Z.add_0_r //. }
+  assert (ℓ ∉ dom σ).
+  { intros Hℓ. destruct Hstore_blocks as [HH1 _].
+    destruct (HH1 _ Hℓ) as (γ'&Hγ'). by apply elem_of_lloc_map_pub_locs_1 in Hγ'. }
+  split_and!; auto. exists ζσ. split_and!; eauto.
+  - eapply is_store_blocks_expose_lloc; eauto.
+  - eapply is_store_expose_lloc; eauto.
+Qed.
+
+Lemma lstore_hybrid_repr_freeze_block χ ζfreeze σ ζ γ bb :
+  χ !! γ = Some LlocPrivate →
+  ζ !! γ = Some (Bvblock (Mut, bb)) →
+  lstore_hybrid_repr χ ζfreeze σ ζ →
+  lstore_hybrid_repr χ (<[γ:=Bvblock (Immut, bb)]> ζfreeze) σ
+    (<[γ:=Bvblock (Immut, bb)]> ζ).
+Proof using.
+  intros ? ? (ζσ&->&?&?&?). exists ζσ. split_and!; eauto.
+  - rewrite insert_union_r. 1: done. eapply map_disjoint_Some_r; eauto.
+  - apply map_disjoint_insert_r. split; last done. by eapply map_disjoint_Some_l.
+  - eapply is_store_freeze_lloc; eauto.
+    eapply lookup_union_Some_r; eauto.
+Qed.
+
+Lemma lstore_hybrid_repr_alloc_block χ ζfreeze σ ζ γ blk :
+  χ !! γ = None →
+  ζfreeze !! γ = None →
+  lstore_hybrid_repr χ ζfreeze σ ζ →
+  lstore_hybrid_repr (<[γ:=LlocPrivate]> χ)
+    (<[γ:=blk]> ζfreeze) σ (<[γ:=blk]> ζ).
+Proof using.
+  intros ? Hζγ (ζσ&->&?&?&?). exists ζσ.
+  apply lookup_union_None in Hζγ as [? ?].
+  split_and!.
+  - rewrite insert_union_r//.
+  - apply map_disjoint_insert_r; split; auto.
+  - eapply is_store_blocks_alloc_block; eauto.
+  - eapply is_store_alloc_block; eauto.
+Qed.
+
+Lemma lstore_hybrid_repr_modify_block χ ζfreeze σ ζ γ blk blk' :
+  ζ !! γ = Some blk →
+  mutability blk = Mut →
+  lstore_hybrid_repr χ ζfreeze σ ζ →
+  lstore_hybrid_repr χ (<[γ:=blk']> ζfreeze) σ (<[γ:=blk']> ζ).
+Proof.
+  intros Hγ ? Hh.
+  pose proof (lstore_hybrid_repr_lookup_lloc _ _ _ _ _ _ Hh Hγ) as Hγf.
+  destruct Hh as (ζσ&->&Hdisj&Hstore_blocks&Hstore). exists ζσ. split_and!; eauto.
+  - rewrite insert_union_r; first done. by erewrite map_disjoint_Some_l.
+  - eapply map_disjoint_dom. erewrite dom_insert_lookup; last by eexists.
+    by eapply map_disjoint_dom.
+  - eapply is_store_modify_priv_block; eauto. intros ℓ Vs Hχ Hσ.
+    assert (γ ∉ dom ζσ) as Hnin.
+    { apply elem_of_dom_2 in Hγ. apply map_disjoint_dom in Hdisj. set_solver. }
+    destruct Hstore_blocks as [_ HH2]. apply Hnin, HH2; eauto.
+Qed.
+
+Definition HGH (χ : lloc_map) (σo : option store) (ζ : lstore) : iProp Σ :=
+  ∃ (ζg : lstore) (χg : lloc_map),
+  "HGHζ" ∷ lstore_own_auth ζg ∗
+  "HGHχ" ∷ lloc_own_auth χg ∗
+  "HGHσo" ∷ match σo with
+  | None =>
+    "[-> ->]" ∷ ⌜ζg = ζ ∧ χg = χ⌝
+  | Some σ => ∃ ζfreeze,
+    "HGHσ" ∷ state_interp σ ∗
+    "%HGHζfreeze" ∷ ⌜freeze_lstore ζ ζfreeze⌝ ∗
+    "%HGHζrepr" ∷ ⌜lstore_hybrid_repr χg ζfreeze σ ζg⌝
+  end ∗
+  "HGHχNone" ∷ ([∗ map] _↦ℓ ∈ pub_locs_in_lstore χg ζg, ℓ ↦M/) ∗
+  "%Hχinj" ∷ ⌜expose_llocs χ χg⌝ ∗
+  "%Hother_blocks" ∷ ⌜dom ζ ⊆ dom χ⌝.
+
+Lemma hgh_dom_lstore_sub χ σo ζ : HGH χ σo ζ -∗ ⌜dom ζ ⊆ dom χ⌝.
+Proof using. iNamed 1. eauto. Qed.
+
+Lemma hgh_χ_inj χ ζ : HGH χ None ζ -∗ ⌜lloc_map_inj χ⌝.
+Proof using. iNamed 1. iNamed "HGHσo". iPureIntro. apply Hχinj. Qed.
+
+Lemma hgh_pointsto_has_lloc χ σ ζ ℓ vs :
+  HGH χ (Some σ) ζ -∗
+  ℓ ↦∗ vs -∗
+  ∃ γ, γ ~ℓ~ ℓ.
+Proof using.
+  iIntros "H Hpto". iNamed "H". iNamed "HGHσo".
+  iDestruct (gen_heap_valid with "HGHσ Hpto") as %Hℓ.
+  destruct HGHζrepr as (? & ? & ? & ? & ?).
+  edestruct is_store_blocks_has_loc as (γ & Hχγ & Hγ); eauto; [].
+  iExists γ. by iApply lloc_own_auth_get_pub.
+Qed.
+
+Lemma hgh_block_sim_is_val χ ζ vs lvs :
+  HGH χ None ζ -∗
+  lvs ~~∗ vs -∗
+  ⌜Forall2 (is_val χ ζ) vs lvs⌝.
+Proof using.
+  iNamed 1. iIntros "Hsim". iNamed "HGHσo".
+  iDestruct (block_sim_arr_auth_is_val' with "HGHχ HGHζ Hsim") as %?; eauto.
+  apply lstore_hybrid_repr_refl.
+Qed.
+
+Lemma hgh_block_sim_of χ ζ σ vs lvs :
+  Forall2 (is_val χ ζ) vs lvs →
+  HGH χ (Some σ) ζ -∗
+  lvs ~~∗ vs.
+Proof using.
+  intros Hvs. iNamed 1. iNamed "HGHσo".
+  iApply (block_sim_arr_of_auth' with "HGHχ HGHζ"); eauto.
+  eapply Forall2_impl; first done. intros ? ? ?.
+  eapply is_val_freeze; eauto. eapply is_val_expose_llocs; eauto.
+Qed.
+
+Local Lemma interp_ML_discarded_locs_pub χpub (σ:store) :
+    gen_heap_interp σ
+ -∗ ([∗ map] ℓ ∈ χpub, ℓ ↦M/)
+ -∗ ⌜map_Forall (λ (_ : nat) (ℓ : loc), σ !! ℓ = Some None) χpub⌝.
+Proof using.
+  induction χpub as [|k l χpub Hin IH] using map_ind; iIntros "HH HK".
+  - iPureIntro. apply map_Forall_empty.
+  - iPoseProof (big_sepM_insert) as "[HL _]". 1: apply Hin.
+    iPoseProof ("HL" with "HK") as "[H1 H2]".
+    iPoseProof (IH with "HH H2") as "%HIH".
+    iPoseProof (gen_heap_valid with "HH H1") as "%Hv".
+    iPureIntro. apply map_Forall_insert. 1: done. split; done.
+Qed.
+
+Lemma hgh_discarded_locs_pub χ σ ζ :
+  HGH χ None ζ -∗
+  state_interp σ -∗
+  ⌜map_Forall (λ (_ : nat) (ℓ : loc), σ !! ℓ = Some None) (pub_locs_in_lstore χ ζ)⌝.
+Proof using.
+  iNamed 1. iNamed "HGHσo". iIntros "Hσ".
+  by iApply (interp_ML_discarded_locs_pub with "Hσ HGHχNone").
+Qed.
+
+Lemma hgh_empty :
+  lstore_own_auth ∅ -∗
+  lloc_own_auth ∅ -∗
+  HGH ∅ None ∅.
+Proof using.
+  iIntros "Hζ Hχ". rewrite /HGH /named. iExists ∅, ∅.
+  iFrame. rewrite pub_locs_in_lstore_empty big_sepM_empty.
+  iPureIntro; split_and!; eauto.
+  - by apply expose_llocs_refl.
+  - set_solver.
+Qed.
+
+Lemma hgh_ml_to_mut χ σ ζ ℓ γ vs :
+  HGH χ (Some σ) ζ -∗
+  ℓ ↦∗ vs -∗
+  γ ~ℓ~ ℓ ==∗
+  ∃ lvs,
+    HGH χ (Some (<[ℓ := None]> σ)) ζ ∗
+    lstore_own_elem γ (DfracOwn 1) (Bvblock (Mut, (TagDefault, lvs))) ∗
+    lvs ~~∗ vs.
+Proof using.
+  iIntros "H Hℓ #Hsim". iNamed "H". iNamed "HGHσo".
+  iDestruct (gen_heap_valid with "HGHσ Hℓ") as %Hσℓ.
+  iDestruct (lloc_own_pub_of with "HGHχ Hsim") as %Hχγ.
+  iAssert (⌜ζg !! γ = None⌝)%I with "[HGHχNone Hℓ]" as %Hζγ.
+  { destruct (ζg !! γ) as [b|] eqn:Hb; [iExFalso|done].
+    iDestruct (big_sepM_lookup with "HGHχNone") as "Hℓ'".
+    { eapply pub_locs_in_lstore_lookup; eauto. eapply elem_of_dom; eauto. }
+    by iDestruct (gen_heap.mapsto_agree with "Hℓ Hℓ'") as %?. }
+  edestruct lstore_hybrid_repr_lookup_loc as (lvs & Hζfγ & Hlvs); eauto; [].
+  iAssert (lvs ~~∗ vs) as "#Hblock".
+  1: by iApply (block_sim_arr_of_auth' with "HGHχ HGHζ").
+  iMod (gen_heap_update _ _ _ None with "HGHσ Hℓ") as "[HGHσ Hℓ]".
+  iMod (lstore_own_insert _ γ (Bvblock (Mut, _)) with "HGHζ") as "(HGHζ & Hz)";
+    first done.
+  iModIntro. iExists lvs. iFrame "Hblock Hz".
+  rewrite /HGH /named. iExists _, _. iFrame. iSplit. 2: iSplit.
+  2: { rewrite (pub_locs_in_lstore_insert_lstore_pub _ _ _ ℓ) //.
+       iApply big_sepM_insert; eauto. by iFrame. }
+  all: iPureIntro; eauto.
+  { eexists. split; eauto. eapply lstore_hybrid_repr_ml_to_mut; eauto. }
+Qed.
+
+Lemma hgh_mut_to_ml χ σ ζ ℓ γ lvs vs :
+  HGH χ (Some σ) ζ -∗
+  lstore_own_elem γ (DfracOwn 1) (Bvblock (Mut, (TagDefault, lvs))) -∗
+  γ ~ℓ~ ℓ -∗
+  lvs ~~∗ vs
+  ==∗
+  HGH χ (Some (<[ℓ:=Some vs]> σ)) ζ ∗
+  ℓ ↦∗ vs.
+Proof using.
+  iIntros "H Hγ #Hsim #Hblksim". iNamed "H". iNamed "HGHσo".
+  iDestruct (lloc_own_pub_of with "HGHχ Hsim") as %Hγℓ.
+  iDestruct (lstore_own_elem_of with "HGHζ Hγ") as %Hζγ.
+  iAssert (⌜σ !! ℓ = Some None⌝)%I with "[Hγ HGHχNone HGHσ]" as %Hσℓ.
+  { iDestruct (big_sepM_lookup with "HGHχNone") as "Hℓ".
+    { eapply pub_locs_in_lstore_lookup; eauto. eapply elem_of_dom; eauto. }
+    by iDestruct (gen_heap_valid with "HGHσ Hℓ") as %?. }
+  iDestruct (block_sim_arr_auth_is_val' with "HGHχ HGHζ Hblksim") as %Hsim;
+    try done; [].
+  iDestruct (big_sepM_delete _ _ _ ℓ with "HGHχNone") as "[Hℓ HGHχNone]".
+  { eapply pub_locs_in_lstore_lookup; eauto. eapply elem_of_dom; eauto. }
+  iMod (gen_heap_update _ _ _ (Some vs) with "HGHσ Hℓ") as "[HGHσ Hℓ]".
+  iDestruct (lstore_own_elem_to_mut with "Hγ") as "Hγ"; first done.
+  iMod (lstore_own_delete with "HGHζ Hγ") as "HGHζ".
+  iModIntro. iFrame "Hℓ". rewrite /HGH /named.
+  iExists _, _. iFrame. iSplit. 2: iSplit.
+  2: by rewrite pub_locs_in_lstore_delete_lstore //.
+  all: iPureIntro; eauto.
+  { exists ζfreeze. split; eauto. eapply lstore_hybrid_repr_mut_to_ml; eauto. }
+Qed.
+
+Lemma hgh_expose_lloc χ σ ζ γ :
+  HGH χ (Some σ) ζ -∗ γ ~ℓ~/ ==∗
+  ∃ ℓ, ⌜ℓ ∉ dom σ⌝ ∗ HGH χ (Some (<[ℓ:=None]> σ)) ζ ∗ γ ~ℓ~ ℓ.
+Proof using.
+  iIntros "H Hpriv". iNamed "H". iNamed "HGHσo".
+  iDestruct (lloc_own_priv_of with "HGHχ Hpriv") as %Hχγ.
+  edestruct lstore_hybrid_repr_expose_lloc as (ℓ & Hℓ & Hℓσ & Hrepr); eauto; [].
+  iMod (lloc_own_expose with "HGHχ Hpriv") as "[HGHχ Hpriv]".
+  iMod (gen_heap_alloc _ ℓ None with "HGHσ") as "(HGHσ & HℓNone & _)".
+  1: by eapply not_elem_of_dom_1.
+  iPoseProof (big_sepM_insert _ _ γ ℓ with "[$HGHχNone $HℓNone]") as "HGHχNone".
+  { eapply map_filter_lookup_None. left. eapply lloc_map_pubs_lookup_None; eauto. }
+  iModIntro. iExists ℓ. iSplit; first done. iFrame "Hpriv". rewrite /HGH /named.
+  iExists _, _. iFrame. iSplit. 2: iSplit.
+  2: iApply (big_sepM_subseteq with "HGHχNone");
+    eapply pub_locs_in_lstore_insert_pub_sub.
+  all: iPureIntro; split_and?; eauto.
+  { eapply expose_llocs_trans; first done. eapply expose_llocs_insert; eauto. }
+Qed.
+
+Lemma hgh_freeze_block χ σ ζ γ bb :
+  HGH χ (Some σ) ζ -∗
+  lstore_own_elem γ (DfracOwn 1) (Bvblock (Mut, bb)) -∗
+  γ ~ℓ~/
+  ==∗
+  HGH χ (Some σ) ζ ∗
+  lstore_own_elem γ (DfracOwn 1) (Bvblock (Immut, bb)) ∗
+  γ ~ℓ~/.
+Proof using.
+  iIntros "H Hγ Hfresh". iNamed "H". iNamed "HGHσo".
+  iDestruct (lstore_own_elem_of with "HGHζ Hγ") as %?.
+  iDestruct (lloc_own_priv_of with "HGHχ Hfresh") as %?.
+  iDestruct (lstore_own_elem_to_mut with "Hγ") as "Hγ"; first done.
+  iMod (lstore_own_update _ _ _ (Bvblock (Immut, bb)) with "HGHζ Hγ") as "(HGHζ & Hγ)".
+  iModIntro. iFrame "Hγ Hfresh". rewrite /HGH /named. iExists _, _. iFrame.
+  iSplit. 2: iSplit.
+  2: { rewrite pub_locs_in_lstore_insert_existing; eauto. by eapply elem_of_dom_2. }
+  all: iPureIntro; eauto.
+  { exists (<[γ:=Bvblock (Immut, bb)]> ζfreeze). split.
+    { eapply freeze_lstore_freeze_lloc; eauto.
+      by eapply lstore_hybrid_repr_lookup_lloc. }
+    { eapply lstore_hybrid_repr_freeze_block; eauto. } }
+Qed.
+
+Lemma hgh_alloc_block χ σ ζ γ blk :
+  χ !! γ = None →
+  HGH χ (Some σ) ζ ==∗
+  HGH (<[γ := LlocPrivate]> χ) (Some σ) (<[γ := blk]> ζ) ∗
+  lstore_own_elem γ (DfracOwn 1) blk ∗
+  γ ~ℓ~/.
+Proof using.
+  intros Hχγ. iNamed 1. iNamed "HGHσo". pose proof Hχinj as [? _].
+  assert (dom ζg ⊆ dom χ).
+  { rewrite <-Hother_blocks. destruct HGHζfreeze as [-> _].
+    destruct HGHζrepr as (?&->&_&_&_). set_solver. }
+  iMod (lstore_own_insert _ γ blk with "HGHζ") as "(HGHζ & Hb)".
+  1: by not_elem_of_dom.
+  assert (Hχg: χg !! γ = None) by not_elem_of_dom.
+  iMod (lloc_own_allocate _ γ with "[%] HGHχ") as "(HGHχ&Hpriv)"; first auto.
+  iModIntro. iFrame "Hpriv Hb". rewrite /HGH /named.
+  iExists _, _. iFrame. iSplit. 2: iSplit.
+  2: rewrite pub_locs_in_lstore_alloc_priv; eauto.
+  all: iPureIntro.
+  { exists (<[γ := blk]> ζfreeze). split.
+    { by eapply freeze_lstore_insert. }
+    { eapply lstore_hybrid_repr_alloc_block; eauto.
+      destruct HGHζfreeze as [? _]. not_elem_of_dom. } }
+  { split; last set_solver. eapply expose_llocs_insert_both; eauto. }
+Qed.
+
+Lemma hgh_lookup_block χ σo ζ γ dq b :
+  HGH χ σo ζ -∗
+  lstore_own_elem γ dq b -∗
+  ⌜∃ b', freeze_block b' b ∧ ζ !! γ = Some b'⌝.
+Proof using.
+  iNamed 1. iIntros "Hγ".
+  iDestruct (lstore_own_elem_of with "HGHζ Hγ") as %Hγ.
+  destruct σo as [σ|]; iNamed "HGHσo"; last by eauto.
+  destruct HGHζfreeze as [H1 H2].
+  eapply lstore_hybrid_repr_lookup_lloc in Hγ; last eassumption.
+  enough (is_Some (ζ !! γ)) as [b' Hb']; first by eauto.
+  apply elem_of_dom. apply elem_of_dom_2 in Hγ. set_solver.
+Qed.
+
+Lemma hgh_lookup_vblock χ σo ζ γ dq m bb :
+  HGH χ σo ζ -∗
+  lstore_own_elem γ dq (Bvblock (m, bb)) -∗
+  ⌜∃ m', (m' = Immut → m = Immut) ∧ ζ !! γ = Some (Bvblock (m', bb))⌝.
+Proof using.
+  iIntros "H Hγ". iDestruct (hgh_lookup_block with "H Hγ") as %(?&Hfrz&?).
+  inversion Hfrz; subst; eauto. iPureIntro; eexists. split; last by eauto.
+  congruence.
+Qed.
+
+Lemma hgh_modify_block χ σ ζ γ blk blk' :
+  mutability blk = Mut →
+  HGH χ (Some σ) ζ -∗
+  lstore_own_elem γ (DfracOwn 1) blk ==∗
+  HGH χ (Some σ) (<[γ := blk']> ζ) ∗
+  lstore_own_elem γ (DfracOwn 1) blk'.
+Proof using.
+  intros Hmut. iNamed 1. iNamed "HGHσo". iIntros "Hpto".
+  iDestruct (lstore_own_elem_of with "HGHζ Hpto") as %Hγ.
+  iDestruct (lstore_own_elem_to_mut with "Hpto") as "Hpto"; auto.
+  iMod (lstore_own_update _ _ _ blk' with "HGHζ Hpto") as "[HGHζ Hpto]".
+  iModIntro. iFrame "Hpto". rewrite /HGH /named.
+  repeat iExists _. iFrame. iSplit. 2: iSplit.
+  2: { rewrite pub_locs_in_lstore_insert_existing //. by eapply elem_of_dom_2. }
+  all: iPureIntro.
+  { eexists. split; first by apply freeze_lstore_insert.
+    eapply lstore_hybrid_repr_modify_block; eauto. }
+  { split; eauto. rewrite dom_insert_L subseteq_union_1_L// singleton_subseteq_l.
+    eapply lstore_hybrid_repr_lookup_lloc in HGHζrepr; last apply Hγ.
+    destruct HGHζfreeze. apply elem_of_dom_2 in HGHζrepr. set_solver. }
+Qed.
+
+Lemma hgh_export_ml_heap χ σ ζ :
+  HGH χ (Some σ) ζ -∗
+  ∃ ζ' χ' ζfreeze,
+    HGH χ' None ζ' ∗
+    state_interp σ ∗
+    ⌜expose_llocs χ χ'⌝ ∗
+    ⌜freeze_lstore ζ ζfreeze⌝ ∗
+    ⌜lstore_hybrid_repr χ' ζfreeze σ ζ'⌝.
+Proof using.
+  iNamed 1. iNamed "HGHσo".
+  iExists ζg, χg, ζfreeze. iFrame. iSplit; last by eauto.
+  rewrite /HGH /named. iExists _, _. iFrame. iPureIntro; split_and!; eauto.
+  { eapply expose_llocs_refl; eauto. }
+  { destruct Hχinj as [Hdom1 _]. rewrite -Hdom1. transitivity (dom ζ); auto.
+    destruct HGHζfreeze as [Hdom2 _]. rewrite Hdom2.
+    destruct HGHζrepr as (?&->&_&_&_). set_solver. }
+Qed.
+
+Lemma hgh_import_ml_interp χold σ ζold χ ζ ζnewimm :
+  lloc_map_mono χold χ →
+  lstore_hybrid_repr χ ζ σ (ζold ∪ ζnewimm) →
+  is_private_blocks χ ζnewimm →
+  dom ζ ⊆ dom χ →
+  ζold ##ₘ ζnewimm →
+  HGH χold None ζold -∗
+  state_interp σ ==∗
+  HGH χ (Some σ) ζ.
+Proof using.
+  intros Hχ Hstore Hpriv Hsub Hdisj.
+  iNamed 1. iNamed "HGHσo". iIntros "Hσ".
+  iMod (lstore_own_insert_many _ ζnewimm with "HGHζ") as "(HGHζ & HGHζnewimm)";
+    first done.
+  iMod (lloc_own_mono with "HGHχ") as "HGHχ"; first done.
+  iModIntro. rewrite /HGH /named. iExists _, _. iFrame. iSplit. 2: iSplit.
+  2: { rewrite pub_locs_in_lstore_insert_priv_store //.
+       erewrite pub_locs_in_lstore_mono at 1; [| eauto..]; []. iFrame. }
+  all: iPureIntro; split_and?; eauto.
+  { eexists. split; eauto. apply freeze_lstore_refl. }
+  { apply expose_llocs_refl; eauto. }
+Qed.
+
+End HGH.
