theories/interop/wp_boundary_laws.v
@@ -9,7 +9,7 @@ From transfinite.base_logic.lib Require Import ghost_map ghost_var.
 From iris.proofmode Require Import proofmode.
 From melocoton.c_interface Require Import defs resources.
 From melocoton.ml_lang Require Import lang lang_instantiation primitive_laws.
-From melocoton.interop Require Import weakestpre wp_utils.
+From melocoton.interop Require Import weakestpre wp_utils hybrid_ghost_heap.
 Import Wrap.
 
 (** lemmas to switch between the ML<->C state interp at a boundary *)
@@ -35,20 +35,26 @@ Proof using.
   iIntros (Hlv) "Hσ HGC Hnb #Hblk".
   iNamed "Hσ". iNamed "SIC". iNamed "HGC". simplify_eq. SI_GC_agree.
 
-  iAssert (⌜Forall2 (is_val χvirt (ζσ ∪ ζvirt)) vs lvs⌝)%I as "%Hval".
-  1: by iApply (block_sim_arr_auth_is_val with "GCχvirt GCζvirt Hblk").
   iAssert (⌜∀ k lv, roots_m !! k = Some lv →
             ∃ w, mem !! k = Some (Storing w) ∧ repr_lval (θC ρc) lv w⌝)%I as "%Hroots".
   1: { iIntros (kk vv Hroots).
        iPoseProof (big_sepM_lookup with "GCrootspto") as "(%wr & Hwr & %Hw2)"; first done.
        iExists wr. iSplit; last done. iApply (gen_heap_valid with "HσC Hwr"). }
   apply map_Forall_lookup_2 in Hroots.
-  destruct (make_repr (θC ρc) roots_m mem) as [privmem Hpriv]; try done.
+  destruct (make_repr (θC ρc) roots_m mem) as [privmem Hpriv]; try done; [].
 
+  iDestruct (hgh_export_ml_heap with "GCHGH")
+    as (ζ' χ' ζfreeze) "(GCHGH & Hσ & %Hχ & %Hfrz & %Hζ)".
+  iAssert (⌜Forall2 (is_val χ' ζfreeze) vs lvs⌝)%I as %Hval.
+  { iDestruct (hgh_block_sim_is_val with "GCHGH Hblk") as %Hval. iPureIntro.
+    eapply Forall2_impl; first done. intros ? ?. eapply is_val_mono; eauto.
+    by eapply lstore_hybrid_repr_lstore_sub. }
+
+  (* TODO: refactor opsem to use lstore_hybrid_repr? *)
+  destruct Hζ as (ζσ&?&?&?&?).
   iExists (WrapstateML _ _ _ _), _. iSplit.
   { iPureIntro. unfold c_to_ml. cbn.
-    eexists σMLvirt, _, _, (ζσ ∪ ζvirt), ζσ. split_and!; eauto.
-    by rewrite map_union_comm. }
+    eexists σMLvirt, _, _, ζfreeze, ζσ. split_and!; eauto. by rewrite map_union_comm. }
 
   iMod (ghost_var_update_halves with "Hnb SIbound") as "(Hb & SIbound)".
   iMod (ghost_var_update_halves with "GCζ SIζ") as "(GCζ & SIζ)".
@@ -58,12 +64,10 @@ Proof using.
   iMod (set_to_none with "HσC GCrootspto") as "(HσC & GCrootspto)"; first done.
 
   iModIntro. iSplitR "SIbound"; last by iFrame "SIbound".
-  rewrite /= /named. iFrame "GCσMLv".
-  unfold private_state_interp, ML_state_interp, GC_token_remnant, named; cbn.
-  iFrame. iPureIntro; split_and!.
-  1: destruct Hχvirt as (_ & HHH); apply HHH.
-  1: apply Hother_blocks.
-  1: destruct Hpriv as (mem_r & ->%repr_roots_dom & Hpriv2 & Hpriv3); by apply map_disjoint_dom.
+  rewrite /= /named. iFrame "Hσ".
+  unfold private_state_interp, ML_state_interp, GC_remnant, named; cbn.
+  iFrame. iPureIntro.
+  destruct Hpriv as (mem_r & ->%repr_roots_dom & Hpriv2 & Hpriv3); by apply map_disjoint_dom.
 Qed.
 
 Lemma wrap_interp_ml_to_c vs ρml σ ws ρc mem :
@@ -82,44 +86,30 @@ Proof using.
                     Hstore & Hvals & ? & ? & ? & Hroots & ?).
 
   iNamed "Hst". iNamed "SIML". iNamed "SIGCrem".
-  iDestruct (ghost_var_split _ _ (1/2) (1/2) with "[SIinit]") as "[SIinit GCinit]".
-  { rewrite {1}(_: 1 = 1/2+1/2)%Qp // Qp.half_half //. }
+  iDestruct (hgh_dom_lstore_sub with "GCHGH") as %Hζsub.
   iMod (ghost_var_update_halves with "Hb SIbound") as "(Hnb & SIbound)".
   iMod (ghost_var_update_halves with "SIζ GCζ") as "(SIζ & GCζ)".
   iMod (ghost_var_update_halves with "SIχ GCχ") as "(SIχ & GCχ)".
   iMod (ghost_var_update_halves with "SIθ GCθ") as "(SIθ & GCθ)".
   iMod (ghost_var_update_halves with "SIroots GCroots") as "(SIroots & GCroots)".
   apply map_disjoint_union_r in Hζdisj as [Hζdisj1 Hζdisj2].
-  iMod (lstore_own_insert_many with "SIζvirt") as "(SIζvirt & SIζnewimm)"; first done.
-  iMod (lloc_own_mono with "SIAχ") as "SIAχ"; first done.
-  assert (ζσ ##ₘ ζnewimm) as Hdisj2 by by eapply is_store_blocks_is_private_blocks_disjoint.
-  assert (ζC ρc = ζσ ∪ (ζML ρml ∪ ζnewimm)) as H6B.
-  1: { rewrite map_union_assoc. rewrite (map_union_comm ζσ); first done. by symmetry. }
-  iPoseProof (block_sim_arr_of_auth _ _ _ _ _ vs lvs with "SIAχ SIζvirt") as "#Hsim".
-  5: eassumption. 1-3:done. 1: by apply map_disjoint_union_r.
+  iMod (hgh_import_ml_interp _ _ _ _ (ζC ρc) with "GCHGH HσML") as "GCHGH"; eauto.
+  (* TODO: use lstore_hybrid_repr in the opsem? *)
+  { exists ζσ. split_and!; eauto.
+    { rewrite map_union_assoc. rewrite (map_union_comm ζσ); first done. by symmetry. }
+    { apply map_disjoint_union_r; split; eauto.
+      by eapply is_store_blocks_is_private_blocks_disjoint. } }
+  { rewrite HζC !dom_union_L. repeat apply union_least.
+    { destruct Hmono as [?%subseteq_dom ?]. set_solver. }
+    { eapply is_store_blocks_lstore_dom_sub; eauto. }
+    { eapply is_private_blocks_dom_sub; eauto. } }
   iMod (set_to_some with "HσCv GCrootspto") as "(HσCv & GCrootspto)"; first done.
+  iDestruct (hgh_block_sim_of _ _ _ vs lvs with "GCHGH") as "#Hsim"; first eassumption.
 
   iModIntro. iFrame "Hnb". rewrite /= /named.
   iFrame "HσCv SIζ SIχ SIθ SIroots SIbound".
-  iSplitL "SIinit". { iExists false. iFrame. }
-  iSplit.
-  { rewrite /GC /named.
-    iExists (ζC ρc), (ζC ρc), ζσ, (ζML ρml ∪ ζnewimm).
-    iExists (χC ρc), (χC ρc), σ, (rootsC ρc), (rootsML ρml).
-    iFrame. iSplit.
-    { rewrite pub_locs_in_lstore_insert_priv_store; last done.
-      erewrite pub_locs_in_lstore_mono at 1; [| eauto..]; [].
-      iFrame "SIAχNone". }
-    iPureIntro; split_and!; eauto.
-    { reflexivity. }
-    { by apply map_disjoint_union_r. }
-    { rewrite dom_union_L. apply union_least.
-      - etransitivity; [ eapply Hother_blocks |].
-        eapply subseteq_dom, Hmono.
-      - eapply elem_of_subseteq. intros γ Hγ.
-        by eapply elem_of_dom_2, Hprivblocks. }
-    { split; first done. split; first apply Hmono.
-      intros γ v1 v2 HH1 HH2. simplify_map_eq. econstructor. } }
+  iSplitL "SIinit". { iExists false. iFrame. } iSplit.
+  { rewrite /GC /named. iExists _, _, _, _, _. iFrame. iPureIntro; split_and!; eauto. }
   { iExists _; by iFrame "Hsim". }
 Qed.
 
