theories/interop/wp_prims/alloc_foreign.v
@@ -21,7 +21,6 @@ Context `{!wrapperG Σ}.
 Implicit Types P : iProp Σ.
 Import mlanguage.
 
-(* TODO: refactor to share proof with wp_prim_alloc *)
 Lemma alloc_foreign_correct e : |- wrap_prog e :: alloc_foreign_proto.
 Proof using.
   iIntros (? ? ? ?) "H". unfold mprogwp. iNamed "H".
@@ -56,71 +55,22 @@ Proof using.
                   HγNone & -> & -> & HGCOK' & Hrepr' & Hrootslive' & ?)).
   destruct_and!; simplify_eq.
 
-  assert (χvirt !! γ = None) as Hχvirtγ.
-  { eapply not_elem_of_dom. destruct Hχvirt as [<- _].
-    by eapply not_elem_of_dom. }
-  assert (ζσ !! γ = None) as Hζσγ.
-  { eapply not_elem_of_dom. destruct Hstore_blocks as [HHL HHR].
-    intros (ℓ&Vs&HX1&HX2)%HHR. congruence. }
-  assert (ζvirt !! γ = None) as Hζvirtγ.
-  { eapply not_elem_of_dom. intros H. eapply not_elem_of_dom in Hχvirtγ.
-    apply Hχvirtγ. eapply elem_of_weaken; first done. done. }
-  assert (ζC ρc !! γ = None) as HζCγ.
-  { destruct Hfreezeρ as [HL HR]. eapply not_elem_of_dom. rewrite HL.
-    rewrite dom_union_L.
-    intros [HH|HH]%elem_of_union.
-    all: eapply elem_of_dom in HH; destruct HH as [v HHv]; congruence. }
-
-  assert (freeze_lstore (<[γ := Bforeign None]> (ζC ρc)) (ζσ ∪ <[γ:=Bforeign None]> ζvirt)) as Hfreezeρ_new.
-  { destruct Hfreezeρ as [HfL HfR]; split.
-    - rewrite !dom_insert_L HfL dom_union_L. set_solver+.
-    - rewrite <- insert_union_r. 2: done.
-      intros γ1 b1 b2 ?%lookup_insert_Some ?%lookup_insert_Some.
-      destruct_or!; destruct_and!; simplify_eq; eauto. }
-
+  iMod (hgh_alloc_block with "GCHGH") as "(GCHGH & Hpto & Hfresh)"; first eassumption.
   iMod (set_to_none _ _ _ _ Hpriv with "HσC GCrootspto") as "(HσC&GCrootspto)".
   iMod (set_to_some _ _ _ _ Hrepr' with "HσC GCrootspto") as "(HσC&GCrootspto)".
-
   iMod (ghost_var_update_halves with "GCζ SIζ") as "(GCζ&SIζ)".
   iMod (ghost_var_update_halves with "GCχ SIχ") as "(GCχ&SIχ)".
   iMod (ghost_var_update_halves with "GCθ SIθ") as "(GCθ&SIθ)".
-
-  iMod (lstore_own_insert _ γ (Bforeign None) with "GCζvirt") as "(GCζvirt & Hbp1)". 1: done.
-  iMod (lloc_own_allocate _ γ with "[] GCχvirt") as "(GCχvirt&Hbp2)". 1: done.
 
   do 3 iModIntro. iFrame. cbn -[wrap_prog].
   iSplitL "SIinit". { iExists false. iFrame. }
   iApply wp_value; first done.
   iApply "Hcont". iFrame.
-  iApply ("Cont" $! θC' γ with "[-Hbp2 Hbp1] [Hbp2 Hbp1] []"); try done.
+  iApply ("Cont" $! θC' γ with "[-Hpto Hfresh] [Hpto Hfresh] []"); try done.
   3: iPureIntro; by econstructor.
   2: iFrame; by eauto.
   rewrite /GC /named.
-  iExists _, _, (ζσ), (<[γ:=Bforeign None]> ζvirt), _, (<[γ:=LlocPrivate]> χvirt).
-  iExists σMLvirt, _, _.
-  rewrite pub_locs_in_lstore_alloc_priv //. iFrame.
-  iPureIntro; split_and!; eauto.
-  2: destruct Hstore_blocks as [HsL HsR]; split.
-  - eapply map_disjoint_insert_r. split; done.
-  - intros ℓ Hdom. destruct (HsL ℓ Hdom) as (γ1 & Hγ1). exists γ1. rewrite lookup_insert_ne; first done.
-    intros ->; congruence.
-  - intros γ1; split.
-    + intros (ℓ&Vs&HH1&HH2)%HsR. exists ℓ,Vs; split; try done.
-      rewrite lookup_insert_ne; first done. intros ->; congruence.
-    + intros (ℓ&Vs&[[??]|[??]]%lookup_insert_Some&HH2); try congruence.
-      eapply HsR. by exists ℓ,Vs.
-  - erewrite !dom_insert_L. clear -Hother_blocks. set_solver.
-  - intros ℓ vs γ1 blk1 HH1 [[??]|[? HH2]]%lookup_insert_Some HH3; try congruence.
-    rewrite -!insert_union_r in HH3|-*; try done.
-    rewrite lookup_insert_ne in HH3; last done.
-    specialize (Hstore ℓ vs γ1 blk1 HH1 HH2 HH3).
-    inversion Hstore; subst. econstructor.
-    eapply Forall2_impl; first eassumption.
-    intros vml vl HH4. eapply is_val_mono. 3: apply HH4.
-    + eapply insert_subseteq. done.
-    + eapply insert_subseteq. eapply lookup_union_None; done.
-  - apply expose_llocs_insert_both; eauto.
-  - eapply GC_correct_transport; done.
+  iExists _, _, σMLvirt, _, _. iFrame; eauto.
 Qed.
 
 End Laws.
