theories/interop/wp_prims/modify.v
@@ -29,68 +29,31 @@ Proof using.
   rewrite weakestpre.wp_unfold. rewrite /weakestpre.wp_pre.
   iIntros "%σ Hσ". cbn -[wrap_prog].
   SI_at_boundary. iNamed "HGC". SI_GC_agree.
-  iDestruct (lstore_own_vblock_mutable_as_mut with "Hpto") as "(Hpto & Hptoacc)";
+  iDestruct (lstore_own_vblock_mutable_as_mut with "Hpto") as "([Hpto _] & Hptoacc)";
     first done.
-  iPoseProof (lstore_own_mut_of with "GCζvirt Hpto") as "%Helem". destruct Helem as [Helem _].
-  iAssert ⌜ζC ρc !! γ = Some (Bvblock (Mut, (tg, vs0)))⌝%I as "%Helem2".
-  1: { iPureIntro. eapply lookup_union_Some_r in Helem; last apply Hfreezedj.
-       destruct Hfreezeρ as [HL HR].
-       assert (γ ∈ dom (ζC ρc)) as [v Hv]%elem_of_dom by by (rewrite HL; eapply elem_of_dom_2).
-       specialize (HR _ _ _ Hv Helem) as Hinv. inversion Hinv; subst; done. }
-
+  iPoseProof (hgh_lookup_block with "GCHGH Hpto") as (b') "(%Hfrz & %Helem)".
+  assert (b' = Bvblock (Mut, (tg, vs0))) as -> by (inversion Hfrz; eauto); clear Hfrz.
   iApply wp_pre_cases_c_prim; [done..|].
-  assert (∃ blk', modify_block (Bvblock (Mut, (tg, vs0))) (Z.to_nat i) v' blk')
-    as (blk'&Hblk').
-  { eexists. eapply mk_modify_block. lia. }
+  set (blk' := Bvblock (Mut, (tg, <[Z.to_nat i := v']> vs0))).
+  assert (modify_block (Bvblock (Mut, (tg, vs0))) (Z.to_nat i) v' blk')
+    by (constructor; lia).
 
   iExists (λ '(e', σ'),
     e' = WrSE (ExprV #0) ∧
     σ' = CState {| χC := χC ρc; ζC := <[γ:=blk']> (ζC ρc); θC := θC ρc; rootsC := rootsC ρc |} mem).
   iSplit. { iPureIntro; econstructor; eauto. }
   iIntros (? ? ? (? & ?)); simplify_eq.
-
-  destruct HGCOK as [HGCL HGCR].
-  iMod (lstore_own_update _ _ _ blk' with "GCζvirt Hpto") as "(GCζvirt&Hpto)".
   iMod (ghost_var_update_halves with "SIζ GCζ") as "(SIζ&GCζ)".
-  iPoseProof (interp_ML_discarded_locs_pub with "GCσMLv GCχNone") as "%Hpublocs".
+  iMod (hgh_modify_block with "GCHGH Hpto") as "[GCHGH Hpto]"; first done.
   do 3 iModIntro. iFrame. iSplitL "SIinit". { iExists false. iFrame. }
   iApply wp_value; first done.
   change (Z.of_nat 0) with (Z0).
   iApply "Hcont". iFrame.
   iApply ("Cont" with "[-Hpto Hptoacc] [Hpto Hptoacc]").
-  { iExists _, (<[γ:=blk']> (ζσ ∪ ζvirt)), ζσ, (<[γ:=blk']>ζvirt), _, χvirt, σMLvirt.
-    iExists _, _. unfold named. iFrame.
-    erewrite pub_locs_in_lstore_insert_existing; last by eapply elem_of_dom_2. iFrame.
-    iPureIntro; split_and!; eauto; cbn. 1: destruct Hfreezeρ as [HL HR]; split.
-    - by erewrite !dom_insert_L, HL.
-    - intros γ' b1 b2 [[? ?]|[Hne1 H1']]%lookup_insert_Some [[??]|[Hne2 H2']]%lookup_insert_Some; try congruence.
-      1: subst; econstructor.
-      subst. by eapply HR.
-    - rewrite insert_union_r; first done.
-      erewrite map_disjoint_Some_l; done.
-    - eapply map_disjoint_dom. erewrite dom_insert_lookup; last by eexists. by eapply map_disjoint_dom.
-    - rewrite dom_insert_lookup; last by eexists.
-      done.
-    - intros ℓ Vs γ1 bb H1' H2' [[<- <-]|[Hne H3']]%lookup_insert_Some.
-      -- epose proof (map_Forall_lookup_1 _ _ γ ℓ Hpublocs) as Hpub2. cbn in Hpub2.
-         rewrite Hpub2 in H1'; first congruence.
-         eapply pub_locs_in_lstore_lookup; last apply H2'.
-         eapply elem_of_dom_2; done.
-      -- specialize (Hstore _ _ _ _ H1' H2' H3'); inversion Hstore; subst.
-         econstructor. eapply Forall2_impl; first done.
-         intros x' y HH; eapply is_val_insert_immut; last done.
-         1: erewrite lookup_union_r; first done.
-         1: eapply map_disjoint_Some_l; done. done.
-    - split; first apply HGCL.
-      intros γ0 blk1 γ1 Hγ0 [[??]|[Hne1 Hlu]]%lookup_insert_Some Hlloc.
-      2: by eapply HGCR. simplify_eq. inv_modify_block.
-      apply lval_in_vblock, list_insert_lookup_inv in Hlloc as [HLL|HRR];
-        simplify_map_eq.
-      { inv_repr_lval. by eapply elem_of_dom_2. }
-      { eapply HGCR; eauto. 1: rewrite lookup_union_r //.
-        1: eapply map_disjoint_Some_l; eauto. by constructor. } }
-  {  iApply lstore_own_vblock_mutable_as_mut; eauto. iFrame.
-     iSplit. 1: inv_modify_block; simplify_map_eq. 1: iFrame. eauto. }
+  { rewrite /GC /named /=. iExists (<[γ:=blk']> (ζC ρc)), _, _, _, _.
+    iFrame. iPureIntro; split_and!; eauto.
+    eapply GC_correct_modify_block; eauto. }
+  { iApply lstore_own_vblock_mutable_as_mut; eauto. by iFrame. }
 Qed.
 
 End Laws.
