theories/interop/wp_prims/write_foreign.v
@@ -23,19 +23,15 @@ Import mlanguage.
 
 Lemma write_foreign_correct e : |- wrap_prog e :: write_foreign_proto.
 Proof using.
-  (* TODO: refactor to share lemmas with prim_modify *)
   iIntros (? ? ? ?) "H". unfold mprogwp. iNamed "H".
   iSplit; first done.
   iIntros (Φ') "Hb Hcont". iApply wp_wrap_call; first done. cbn [snd].
   rewrite weakestpre.wp_unfold. rewrite /weakestpre.wp_pre.
   iIntros "%σ Hσ". cbn -[wrap_prog].
   SI_at_boundary. iNamed "HGC". SI_GC_agree.
-  iDestruct (lstore_own_mut_of with "GCζvirt Hpto") as %[Helem _].
-  iAssert ⌜ζC ρc !! γ = Some (Bforeign wo)⌝%I as "%Helem2".
-  { iPureIntro. eapply lookup_union_Some_r in Helem; last apply Hfreezedj.
-    eapply freeze_lstore_lookup_backwards in Helem as (?&Hfrz&?); eauto.
-    inversion Hfrz; by simplify_eq. }
-  destruct HGCOK as [HGCL HGCR]. inv_repr_lval.
+  iDestruct "Hpto" as "(Hpto & _)".
+  iPoseProof (hgh_lookup_block with "GCHGH Hpto") as (b) "(%Hb&%Hγ)".
+  inversion Hb; subst; clear Hb.
 
   iApply wp_pre_cases_c_prim; [done..|].
   iExists (λ '(e', σ'),
@@ -43,43 +39,16 @@ Proof using.
     σ' = CState (WrapstateC (χC ρc) (<[γ:=Bforeign (Some w')]> (ζC ρc)) (θC ρc) (rootsC ρc)) mem).
   iSplit. { iPureIntro; econstructor; eauto. }
   iIntros (? ? ? (? & ?)); simplify_eq.
-
-  iMod (lstore_own_update _ _ _ (Bforeign (Some w')) with "GCζvirt Hpto") as "(GCζvirt&Hpto)".
   iMod (ghost_var_update_halves with "SIζ GCζ") as "(SIζ&GCζ)".
-  iPoseProof (interp_ML_discarded_locs_pub with "GCσMLv GCχNone") as "%Hpublocs".
+  iMod (hgh_modify_block with "GCHGH Hpto") as "(GCHGH & Hpto)"; first done.
   do 3 iModIntro. iFrame. cbn -[wrap_prog] in *.
   iSplitL "SIinit". { iExists false. iFrame. }
   iApply wp_value; first done.
   change (Z.of_nat 0) with (Z0).
   iApply "Hcont". iFrame.
-  iApply ("Cont" with "[-Hpto] [$Hpto]").
-  { iExists _, (<[γ:=Bforeign (Some w')]> (ζσ ∪ ζvirt)), ζσ, (<[γ:=Bforeign (Some w')]>ζvirt), _, χvirt, σMLvirt.
-    iExists _, _. unfold named. iFrame.
-    erewrite pub_locs_in_lstore_insert_existing; last by eapply elem_of_dom_2. iFrame.
-    iPureIntro; split_and!; eauto; cbn. 1: destruct Hfreezeρ as [HL HR]; split.
-    - by erewrite !dom_insert_L, HL.
-    - intros γ' b1 b2 [[? ?]|[Hne1 H1']]%lookup_insert_Some [[??]|[Hne2 H2']]%lookup_insert_Some; try congruence.
-      1: subst; econstructor.
-      subst. by eapply HR.
-    - rewrite insert_union_r; first done.
-      erewrite map_disjoint_Some_l; done.
-    - eapply map_disjoint_dom. erewrite dom_insert_lookup; last by eexists. by eapply map_disjoint_dom.
-    - rewrite dom_insert_lookup; last by eexists.
-      done.
-    - intros ℓ Vs γ1 bb H1' H2' [[<- <-]|[Hne H3']]%lookup_insert_Some.
-      -- epose proof (map_Forall_lookup_1 _ _ γ ℓ Hpublocs) as Hpub2. cbn in Hpub2.
-         rewrite Hpub2 in H1'; first congruence.
-         eapply pub_locs_in_lstore_lookup; last apply H2'.
-         eapply elem_of_dom_2; done.
-      -- specialize (Hstore _ _ _ _ H1' H2' H3'); inversion Hstore; subst.
-         econstructor. eapply Forall2_impl; first done.
-         intros x' y HH; eapply is_val_insert_immut; last done.
-         1: erewrite lookup_union_r; first done.
-         1: eapply map_disjoint_Some_l; done. done.
-    - split; first apply HGCL.
-      intros γ0 blk1 γ1 Hγ0 [[??]|[Hne1 Hlu]]%lookup_insert_Some Hlloc.
-      2: by eapply HGCR. simplify_eq. inversion Hlloc. }
-  { done. }
+  iApply ("Cont" with "[-Hpto] [$Hpto//]").
+  rewrite /GC /named. iExists _, _, _, _, _. iFrame. iPureIntro; split_and!; eauto.
+  eapply GC_correct_modify_foreign; eauto.
 Qed.
 
 End Laws.
